Update RISC-V CPUTimingBehavior module to be pedantic about timing, update addloop proof as an example

timing/examples/riscv_addloop_timing_proof.v
@@ -66,31 +66,74 @@ Import Program_addloop addloopAuto.
    the loop condition *must* have fallen through. But after the loop exits,
    we know that the loop condition must have taken the branch.
 *)
-Definition addloop_timing_invs (x y : N) (t:trace) :=
+Definition sum (low high : N) (f : N -> N) : N :=
+    let range := List.map N.of_nat (List.seq (N.to_nat low) (N.to_nat (high - low))) in
+    List.fold_left (fun acc i => acc + f i) range 0.
+
+Lemma sum_0_0 : forall f, sum 0 0 f = 0.
+Proof. reflexivity. Qed.
+
+Lemma sum_Sn : forall low high f,
+    low <= high ->
+    sum low (1 + high) f = sum low high f + f high.
+Proof.
+    intros. unfold sum at 1.
+    rewrite <- N.add_sub_assoc, N.add_1_l, N2Nat.inj_succ.
+    rewrite seq_S, map_app, fold_left_app. simpl.
+    rewrite N2Nat.inj_sub at 2.
+    rewrite Arith_base.le_plus_minus_r_stt by lia.
+    rewrite N2Nat.id. reflexivity. assumption.
+Qed.
+
+Lemma sum_sub1 : forall low high body,
+    low < high ->
+    sum low (high - 1) (fun _ => body) + body = 
+        sum low high (fun _ => body).
+Proof.
+    intros. unfold sum at 2.
+    destruct (high - low) eqn:E using N.peano_ind.
+    - lia.
+    - clear IHn. rewrite N2Nat.inj_succ, seq_S, map_app, fold_left_app.
+      simpl. unfold sum. now replace n with (high - 1 - low) by lia.
+Qed.
+
+Definition addloop_timing_invs (t3 x y : N) (t:trace) :=
 match t with (Addr a, s) :: t' => match a with
-    | 0x8  => Some (s R_T0 = x /\ s R_T1 = y /\
+    | 0x8  => Some (s R_T0 = x /\ s R_T1 = y /\ s R_T3 = t3 /\
         cycle_count_of_trace t' = 0)
-    | 0x10 => Some (s R_T2 = 1 /\ s R_T3 = 0 /\ 
-        s R_T0 <= x /\
+    | 0x10 => Some (s R_T2 = 1 /\ s R_T3 = 0 /\
+        s R_T0 <= x /\ s R_T1 = y ⊕ (x - s R_T0) /\
         cycle_count_of_trace t' = 
-            tori + tandi + (x - s R_T0) * (tfbeq + taddi + tsub + ttbeq))
-        (* 2 + 2 + (x - t0) * (3 + 2 + 2 + (5 + (ML - 1)) *)
+            (tori 0 1) + (tandi t3 0) + 
+            sum 0 (x - s R_T0) (fun i =>
+                tfbeq (x - i) 0 +
+                taddi (y ⊕ i) 1 +
+                tsub (x - i) 1 +
+                ttbeq 0 0
+            ))
     | 0x20 => Some (cycle_count_of_trace t' = 
-            tori + tandi + x * (tfbeq + taddi + tsub + ttbeq) + ttbeq)
+            (tori 0 1) + (tandi t3 0) + 
+            sum 0 x (fun i =>
+                tfbeq (x - i) 0 +
+                taddi (y ⊕ i) 1 +
+                tsub (x - i) 1 +
+                ttbeq 0 0
+            ) + ttbeq 0 0)
         (* 2 + 2 + (5 + (ML - 1)) + x * (3 + 2 + 2 + (5 + (ML - 1))) *)
     | _ => None end
 | _ => None
 end.
 
 Theorem addloop_timing:
-  forall s t s' x' x y
+  forall s t s' x' x y t3
          (ENTRY: startof t (x',s') = (Addr entry_addr,s)) (* Define the entry point of the function *)
          (MDL: models rvtypctx s)
          (T0: s R_T0 = x)                   (* Tie the contents of T0 to x *)
-         (T1: s R_T1 = y),                  (* Tie the contents of T1 to y *)
+         (T1: s R_T1 = y)                  (* Tie the contents of T1 to y *)
+         (T3: s R_T3 = t3),
   satisfies_all 
     lifted_prog                                 (* Provide lifted code *)
-    (addloop_timing_invs x y)                  (* Provide invariant set *)
+    (addloop_timing_invs t3 x y)                  (* Provide invariant set *)
     exits                                   (* Provide exit point *)
   ((x',s')::t).
 Proof.
@@ -116,21 +159,32 @@ Proof.
     destruct_inv 32 PRE.
 
     (* Addr 0x8 *)
-    destruct PRE as [T0 [T2 Cycles]].
-    repeat step. repeat split; try assumption. lia. 
-    hammer.
+    destruct PRE as [T0 [T2 [T3 Cycles]]].
+    repeat step. repeat split; try assumption. lia.
+    subst. rewrite N.sub_diag, N.add_0_r.
+        now rewrite N.mod_small by apply (models_var R_T1 MDL).
+    hammer. rewrite N.sub_diag, sum_0_0. lia.
 
     (* Addr 0x10 *)
-    destruct PRE as [T2 [T3 [T0 Cycles_t]]].
+    destruct PRE as [T2 [T3 [T0 [T1 Cycles_t]]]].
     step.
     - (* t0 = 0 -> postcondition *)
-        hammer.
+        remember (sum 0 x _).
+        hammer. apply N.eqb_eq in BC. rewrite BC, N.sub_0_r.
+        subst n. lia.
     - (* t0 <> 0 -> loop again *)
         step. step. step.
         rewrite msub_nowrap by (psimpl; lia).
-        repeat split.
-            lia.
-        hammer. rewrite N_sub_distr; lia.
+        repeat split; try lia;
+            rewrite (N.mod_small (s' R_T0)) by
+                apply (models_var R_T0 MDL);
+            rewrite (N.mod_small 1) by lia.
+            rewrite N_sub_distr; lia.
+        remember (sum 0 (x - update _ _ _ _) _).
+        hammer. subst n. rewrite update_updated.
+        rewrite N_sub_distr, (N.add_comm _ 1), sum_Sn,
+            N_sub_distr, N.sub_diag, N.add_0_l;
+            auto; try lia. 
 Qed.
 
 End TimingProof.
