timing/riscv/CPUTimingBehavior.v
@@ -2,61 +2,89 @@ Require Import NArith.
 
 Module Type CPUTimingBehavior.
     (* === Instruction Timings === *)
+
+    (* ==== I ISA Extension ==== *)
+    (* ALU: rd rs1 rs2 *)
     Parameter
-        (* ==== I ISA Extension ==== *)
-        (* ALU *)
-            tadd taddi tslt tslti tsltu tsltiu
-            txor txori tor tori tand tandi tsub tlui
-            tauipc
-        (* Branches *)
-            (* taken *)
-                ttbeq ttbne ttblt ttbge ttbltu ttbgeu
-            (* not taken *)
-                tfbeq tfbne tfblt tfbge tfbltu tfbgeu
-        (* Jump/call *)
-            tjal tjalr
-        (* Load/store *)
-            tlb tlh tlw tlbu tlhu tsb tsh tsw
-        (* Data fence *)
-            tfence
-        (* System *)
-            tecall tebreak tmret twfi
-
-        (* ==== M ISA Extension ==== *)
-        (* Multiplication *)
-            tmul tmulh tmulhsu tmulhu
-        (* Division *)
-            tdiv tdivu trem tremu
-
-        (* ==== Zbb ISA Extension ==== *)
-        (* Logic with negate *)
-            tandn torn txnor
-        (* Integer max/min *)
-            tmin tminu tmax tmaxu
-        (* Sign/zero extension *)
-            tsext_b tsext_h tzext
-        (* OR-combine *)
-            torc_b
-        (* Byte-reverse *)
-            trev8
-
-        (* ==== Zicsr ISA Extension ==== *)
-        (* System *)
-            tcsrrw tcsrrwi
-            tcsrrs tcsrrsi
-            tcsrrc tcsrrci
-    : N.
-
-    (* These instr times need to be N->N because they could depend on state values *)
+        tadd tsub tslt tsltu txor tor tand : N -> N -> N.
+    (* ALU (immediate): rd rs1 imm *)
     Parameter
-        (* ==== I ISA Extension ==== *)
-        (* ALU Shifts *)
-            tsll tslli tsrl tsrli tsra tsrai
+        taddi tslti tsltiu txori tori tandi : N -> N -> N.
+    (* Upper immediates: rd imm *)
+    Parameter
+        tlui tauipc : N -> N.
 
-        (* ==== Zbb ISA Extension ==== *)
-        (* Bit count *)
-            tclz tctz tcpop
-        (* Bitwise rotation *)
-            trol tror trori
-    : N -> N.
+    (* Branches: rs1 rs2 imm *)
+    Parameter
+        (* taken *)
+        ttbeq ttbne ttblt ttbge ttbltu ttbgeu
+        (* not taken *)
+        tfbeq tfbne tfblt tfbge tfbltu tfbgeu :
+            N -> N -> N.
+
+    (* Jump/call *)
+    Parameter
+        (* jal: rd imm *)
+        tjal : N -> N.
+    Parameter
+        (* jalr: rd rs1 imm *)
+        tjalr : N -> N -> N.
+
+    (* Load/store *)
+    Parameter
+        (* load: rd rs1 imm *)
+        tlb tlh tlw tlbu tlhu
+        (* store: rs1 rs2 imm *)
+        tsb tsh tsw : N -> N -> N.
+
+    (* Data fence: no operands *)
+    Parameter tfence : N.
+
+    (* System: no operands or immediate *)
+    Parameter
+        tecall tebreak tmret twfi : N.
+
+    (* ==== M ISA Extension ==== *)
+    (* Multiplication/division: rd rs1 rs2 *)
+    Parameter
+        tmul tmulh tmulhsu tmulhu
+        tdiv tdivu trem tremu : N -> N -> N.
+
+    (* ==== Zbb ISA Extension ==== *)
+    (* Logic with negate: rd rs1 rs2 *)
+    Parameter
+        tandn torn txnor : N -> N -> N.
+    (* Integer max/min: rd rs1 rs2 *)
+    Parameter
+        tmin tminu tmax tmaxu : N -> N -> N.
+    (* Sign/zero extension: rd rs1 *)
+    Parameter
+        tsext_b tsext_h tzext : N -> N.
+    (* OR-combine: rd rs1 *)
+    Parameter torc_b : N -> N.
+    (* Byte-reverse: rd rs1 *)
+    Parameter trev8 : N -> N.
+
+    (* ==== Zicsr ISA Extension ==== *)
+    (* System CSR access: rd rs1 csr *)
+    Parameter
+        tcsrrw tcsrrs tcsrrc : N -> N -> N.
+    (* System CSR immediate: rd csr imm *)
+    Parameter
+        tcsrrwi tcsrrsi tcsrrci : N -> N -> N.
+
+    (* ==== I ISA Extension ==== *)
+    (* ALU Shifts: rd rs1 (rs2 or imm) *)
+    Parameter
+        tsll tsrl tsra
+        tslli tsrli tsrai : N -> N -> N.
+
+    (* ==== Zbb ISA Extension ==== *)
+    (* Bit count: rd rs1 *)
+    Parameter
+        tclz tctz tcpop : N -> N.
+    (* Bitwise rotation: rd rs1 (rs2 or imm) *)
+    Parameter
+        trol tror
+        trori : N -> N -> N.
 End CPUTimingBehavior.
